LowParse.Pulse.Array

src/lowparse/pulse/LowParse.Pulse.ArrayPtr.fst
@@ -20,10 +20,12 @@ noeq type array_ptr_step0
         ))
         (ensures v1 == v2);
     arrayptr: (#elt: Type0) -> t elt -> v elt -> vprop;
+(*    
     null: (#elt: Type0) -> t elt;
     arrayptr_not_null: (#elt: Type0) -> (r: t elt) -> (#value: v elt) -> stt_ghost unit emp_inames
         (arrayptr r value)
         (fun _ -> arrayptr r value ** pure (~ (r == null)));
+*)        
     adjacent: (#elt: Type0) -> (x1: array elt) -> (x2: array elt) -> prop;
     merge: (#elt: Type0) -> (x1: array elt) -> (x2: array elt) -> Ghost (array elt)
         (requires (adjacent x1 x2))
@@ -54,6 +56,7 @@ let length
 : GTot nat
 = SZ.v (instance0.len r)
 
+(*
 let arrayptr_or_null
     (#t: Type0 -> Type0)
     (#array: Type0 -> Type0)
@@ -66,6 +69,7 @@ let arrayptr_or_null
 = if FStar.StrongExcludedMiddle.strong_excluded_middle (r == instance0.null)
   then emp
   else instance0.arrayptr r value
+*)
 
 let merge_into
     (#t: Type0 -> Type0)
@@ -78,6 +82,133 @@ let merge_into
 = instance0.adjacent x1 x2 /\
   instance0.merge x1 x2 == y
 
+let arrayptr
+    (#t: Type0 -> Type0)
+    (#array: Type0 -> Type0)
+    (#v: Type0 -> Type0)
+    (instance0: array_ptr_step0 t array v)
+: (#elt: Type0) -> t elt -> v elt -> vprop
+= instance0.arrayptr
+
+unfold
+let gsplit_post
+    (#t: Type0 -> Type0)
+    (#array: Type0 -> Type0)
+    (#v: Type0 -> Type0)
+    (instance0: array_ptr_step0 t array v)
+    (#elt:Type)
+    (x: t elt)
+    (i:SZ.t)
+    (value:v elt)
+    (res: Ghost.erased (t elt))
+    (vl: v elt)
+    (vr: v elt)
+: Tot prop
+=
+    SZ.v i <= length instance0 (instance0.array_of value) /\
+    merge_into instance0 (instance0.array_of vl) (instance0.array_of vr) (instance0.array_of value) /\
+    instance0.contents_of vl == Seq.slice (instance0.contents_of value) 0 (SZ.v i) /\
+    length instance0 (instance0.array_of vl) == SZ.v i /\
+    length instance0 (instance0.array_of vr) == length instance0 (instance0.array_of value) - SZ.v i /\
+    instance0.contents_of vr == Seq.slice (instance0.contents_of value) (SZ.v i) (length instance0 (instance0.array_of value)) /\
+    instance0.contents_of value == instance0.contents_of vl `Seq.append` instance0.contents_of vr /\
+    (SZ.v i == 0 ==> Ghost.reveal res == x)
+
+let join_t
+    (#t: Type0 -> Type0)
+    (#array: Type0 -> Type0)
+    (#v: Type0 -> Type0)
+    (instance0: array_ptr_step0 t array v)
+= (#elt:Type) -> (al: t elt) -> (ar: t elt) -> (#vl: v elt) -> (#vr: v elt) -> stt_ghost (Ghost.erased (v elt)) emp_inames
+        (arrayptr instance0 al vl ** arrayptr instance0 ar vr ** pure (
+            instance0.adjacent (instance0.array_of vl) (instance0.array_of vr)
+        ))
+        (fun res -> arrayptr instance0 al res ** pure (
+            merge_into instance0 (instance0.array_of vl) (instance0.array_of vr) (instance0.array_of res) /\
+            instance0.contents_of res == instance0.contents_of vl `Seq.append` instance0.contents_of vr
+        ))
+
+let gsplit_t
+    (#t: Type0 -> Type0)
+    (#array: Type0 -> Type0)
+    (#v: Type0 -> Type0)
+    (instance0: array_ptr_step0 t array v)
+= (#elt:Type) -> (x: t elt) -> (i:SZ.t) -> (#value:v elt) -> stt_ghost (Ghost.erased (t elt)) emp_inames
+        (arrayptr instance0 x value ** pure (
+            SZ.v i <= length instance0 (instance0.array_of value)
+        ))
+        (fun res -> exists_ (fun vl -> exists_ (fun vr ->
+            arrayptr instance0 x vl ** arrayptr instance0 res vr ** pure (
+                gsplit_post instance0 x i value res vl vr
+        ))))
+
+let split_t
+    (#t: Type0 -> Type0)
+    (#array: Type0 -> Type0)
+    (#v: Type0 -> Type0)
+    (instance0: array_ptr_step0 t array v)
+= (#elt:Type) -> (x: t elt) -> (i: SZ.t) -> (x': Ghost.erased (t elt)) -> (#vl: Ghost.erased (v elt)) -> (#vr: Ghost.erased (v elt)) -> stt (t elt)
+        (arrayptr instance0 x vl ** arrayptr instance0 x' vr ** pure (
+            instance0.adjacent (instance0.array_of vl) (instance0.array_of vr) /\
+            SZ.v i == length instance0 (instance0.array_of vl)
+        ))
+        (fun res -> arrayptr instance0 x vl ** arrayptr instance0 res vr ** pure (
+            res == Ghost.reveal x'
+        ))
+
+let index_t
+    (#t: Type0 -> Type0)
+    (#array: Type0 -> Type0)
+    (#v: Type0 -> Type0)
+    (instance0: array_ptr_step0 t array v)
+= (#elt:Type) -> (r: t elt) -> (i: SZ.t) -> (#value: Ghost.erased (v elt)) -> stt elt
+        (arrayptr instance0 r value ** pure (
+            SZ.v i < length instance0 (instance0.array_of value)
+        ))
+        (fun y -> arrayptr instance0 r value ** pure (
+            SZ.v i < length instance0 (instance0.array_of value) /\
+            y == Seq.index (instance0.contents_of value) (SZ.v i)
+        ))
+
+let upd_t
+    (#t: Type0 -> Type0)
+    (#array: Type0 -> Type0)
+    (#v: Type0 -> Type0)
+    (instance0: array_ptr_step0 t array v)
+= (#elt:Type) -> (r: t elt) -> (i:SZ.t) -> (x:elt) -> (#value: Ghost.erased (v elt)) -> stt (Ghost.erased (v elt))
+        (arrayptr instance0 r value ** pure (
+            SZ.v i < length instance0 (instance0.array_of value) /\
+            instance0.array_perm (instance0.array_of value) == full_perm
+        ))
+        (fun value' -> arrayptr instance0 r value' ** pure (
+            SZ.v i < length instance0 (instance0.array_of value) /\
+            instance0.array_of value' == instance0.array_of value /\
+            instance0.contents_of value' == Seq.upd (instance0.contents_of value) (SZ.v i) x
+        ))
+
+let copy_t
+    (#t: Type0 -> Type0)
+    (#array: Type0 -> Type0)
+    (#v: Type0 -> Type0)
+    (instance0: array_ptr_step0 t array v)
+=       (#elt: Type) ->
+        (ain: t elt) ->
+        (aout: t elt) ->
+        (len: SZ.t) ->
+        (#vin: Ghost.erased (v elt)) ->
+        (#vout: Ghost.erased (v elt)) ->
+        stt (Ghost.erased (v elt))
+            (arrayptr instance0 ain vin ** arrayptr instance0 aout vout ** pure (
+                SZ.v len == length instance0 (instance0.array_of vin) /\
+                SZ.v len == length instance0 (instance0.array_of vout) /\
+                instance0.array_perm (instance0.array_of vout) == full_perm
+            ))
+            (fun vout' -> arrayptr instance0 ain vin ** arrayptr instance0 aout vout' ** pure (
+                instance0.array_of vout' == instance0.array_of vout /\
+                length instance0 (instance0.array_of vin) == length instance0 (instance0.array_of vout) /\
+                instance0.contents_of vout' == instance0.contents_of vin
+            ))
+
 inline_for_extraction
 // class array_ptr_step0
 noeq type array_ptr_step1
@@ -86,58 +217,16 @@ noeq type array_ptr_step1
     (#v: Type0 -> Type0)
     (instance0: array_ptr_step0 t array v)
 = {
+(*
     is_null: (#elt: Type0) -> (r: t elt) -> (#value: Ghost.erased (v elt)) -> stt bool
         (arrayptr_or_null instance0 r value)
         (fun res -> arrayptr_or_null instance0 r value ** pure (res == true <==> r == instance0.null));
-    join: (#elt:Type) -> (al: t elt) -> (ar: t elt) -> (#vl: v elt) -> (#vr: v elt) -> stt_ghost (Ghost.erased (v elt)) emp_inames
-        (instance0.arrayptr al vl ** instance0.arrayptr ar vr ** pure (
-            instance0.adjacent (instance0.array_of vl) (instance0.array_of vr)
-        ))
-        (fun res -> instance0.arrayptr al res ** pure (
-            merge_into instance0 (instance0.array_of vl) (instance0.array_of vr) (instance0.array_of res) /\
-            instance0.contents_of res == instance0.contents_of vl `Seq.append` instance0.contents_of vr
-        ));
-    gsplit: (#elt:Type) -> (x: t elt) -> (i:SZ.t) -> (#value:v elt) -> stt_ghost (Ghost.erased (t elt)) emp_inames
-        (instance0.arrayptr x value ** pure (
-            SZ.v i <= length instance0 (instance0.array_of value)
-        ))
-        (fun res -> exists_ (fun vl -> exists_ (fun vr ->
-            instance0.arrayptr x vl ** instance0.arrayptr res vr ** pure (
-            SZ.v i <= length instance0 (instance0.array_of value) /\
-            merge_into instance0 (instance0.array_of vl) (instance0.array_of vr) (instance0.array_of value) /\
-            instance0.contents_of vl == Seq.slice (instance0.contents_of value) 0 (SZ.v i) /\
-            length instance0 (instance0.array_of vl) == SZ.v i /\
-            length instance0 (instance0.array_of vr) == length instance0 (instance0.array_of value) - SZ.v i /\
-            instance0.contents_of vr == Seq.slice (instance0.contents_of value) (SZ.v i) (length instance0 (instance0.array_of value)) /\
-            instance0.contents_of value == instance0.contents_of vl `Seq.append` instance0.contents_of vr /\
-            (SZ.v i == 0 ==> Ghost.reveal res == x)
-        ))));
-    split': (#elt:Type) -> (x: t elt) -> (i: SZ.t) -> (x': Ghost.erased (t elt)) -> (#vl: Ghost.erased (v elt)) -> (#vr: Ghost.erased (v elt)) -> stt (t elt)
-        (instance0.arrayptr x vl ** instance0.arrayptr x' vr ** pure (
-            instance0.adjacent (instance0.array_of vl) (instance0.array_of vr) /\
-            SZ.v i == length instance0 (instance0.array_of vl)
-        ))
-        (fun res -> instance0.arrayptr x vl ** instance0.arrayptr res vr ** pure (
-            res == Ghost.reveal x'
-        ));
-    index: (#elt:Type) -> (r: t elt) -> (i: SZ.t) -> (#value: Ghost.erased (v elt)) -> stt elt
-        (instance0.arrayptr r value ** pure (
-            SZ.v i < length instance0 (instance0.array_of value)
-        ))
-        (fun y -> instance0.arrayptr r value ** pure (
-            SZ.v i < length instance0 (instance0.array_of value) /\
-            y == Seq.index (instance0.contents_of value) (SZ.v i)
-        ));
-    upd: (#elt:Type) -> (r: t elt) -> (i:SZ.t) -> (x:elt) -> (#value: Ghost.erased (v elt)) -> stt (Ghost.erased (v elt))
-        (instance0.arrayptr r value ** pure (
-            SZ.v i < length instance0 (instance0.array_of value) /\
-            instance0.array_perm (instance0.array_of value) == full_perm
-        ))
-        (fun value' -> instance0.arrayptr r value' ** pure (
-            SZ.v i < length instance0 (instance0.array_of value) /\
-            instance0.array_of value' == instance0.array_of value /\
-            instance0.contents_of value' == Seq.upd (instance0.contents_of value) (SZ.v i) x
-        ));
+*)
+    join: join_t instance0;
+    gsplit: gsplit_t instance0;
+    split': split_t instance0;
+    index: index_t instance0;
+    upd: upd_t instance0;
     set_array_perm: 
         (#elt: Type) ->
         (a: array elt) ->
@@ -168,24 +257,10 @@ noeq type array_ptr_step1
         (ensures (
             merge_into instance0 (set_array_perm a1 p) (set_array_perm a2 p) (set_array_perm (instance0.merge a1 a2) p)
         ));
-    copy:
-        (#elt: Type) ->
-        (ain: t elt) ->
-        (aout: t elt) ->
-        (len: SZ.t) ->
-        (#vin: Ghost.erased (v elt)) ->
-        (#vout: Ghost.erased (v elt)) ->
-        stt (Ghost.erased (v elt))
-            (instance0.arrayptr ain vin ** instance0.arrayptr aout vout ** pure (
-                SZ.v len == length instance0 (instance0.array_of vin) /\
-                SZ.v len == length instance0 (instance0.array_of vout) /\
-                instance0.array_perm (instance0.array_of vout) == full_perm
-            ))
-            (fun vout' -> instance0.arrayptr ain vin ** instance0.arrayptr aout vout' ** pure (
-                instance0.array_of vout' == instance0.array_of vout /\
-                length instance0 (instance0.array_of vin) == length instance0 (instance0.array_of vout) /\
-                instance0.contents_of vout' == instance0.contents_of vin
-            ));
+    copy: copy_t instance0;
+}
+
+(*
     share:
         (#elt: Type) ->
         (a: t elt) ->
@@ -193,10 +268,10 @@ noeq type array_ptr_step1
         (p2: perm) ->
         (#x: Ghost.erased (v elt)) ->
         stt_ghost (Ghost.erased (v elt & v elt)) emp_inames
-            (instance0.arrayptr a x ** pure (
+            (arrayptr instance0 a x ** pure (
                 instance0.array_perm (instance0.array_of x) == p1 `Steel.FractionalPermission.sum_perm` p2
             ))
-            (fun res -> instance0.arrayptr a (fst res) ** instance0.arrayptr a (snd res) ** pure (
+            (fun res -> arrayptr instance0 a (fst res) ** arrayptr instance0 a (snd res) ** pure (
                 instance0.array_of (fst res) == set_array_perm (instance0.array_of x) p1 /\
                 instance0.array_of (snd res) == set_array_perm (instance0.array_of x) p2 /\
                 instance0.contents_of (fst res) == instance0.contents_of x /\
@@ -208,10 +283,10 @@ noeq type array_ptr_step1
         (#x1: Ghost.erased (v elt)) ->
         (#x2: Ghost.erased (v elt)) ->
         stt_ghost (Ghost.erased (v elt)) emp_inames
-            (instance0.arrayptr a x1 ** instance0.arrayptr a x2 ** pure (
+            (arrayptr instance0 a x1 ** arrayptr instance0 a x2 ** pure (
                 instance0.array_of x1 == set_array_perm (instance0.array_of x2) (instance0.array_perm (instance0.array_of x1))
             ))
-            (fun res -> instance0.arrayptr a res ** pure (
+            (fun res -> arrayptr instance0 a res ** pure (
                 instance0.array_of x1 == set_array_perm (instance0.array_of x2) (instance0.array_perm (instance0.array_of x1)) /\
                 instance0.array_of res == set_array_perm (instance0.array_of x1) (instance0.array_perm (instance0.array_of x1) `Steel.FractionalPermission.sum_perm` instance0.array_perm (instance0.array_of x2)) /\
                 instance0.contents_of res == instance0.contents_of x1 /\
