src/lowparse/pulse/LowParse.Pulse.Array.fst
@@ -1,0 +1,389 @@
+module LowParse.Pulse.Array
+module LA = LowParse.Pulse.ArrayPtr
+module A = Pulse.Lib.Array
+module SZ = FStar.SizeT
+open Pulse.Lib.Pervasives
+
+// FIXME: expose array_ptr in Pulse.Lib.Array.Core
+noeq
+type t elt = {
+    base: A.array elt;
+    glen: (glen: Ghost.erased SZ.t {SZ.v glen == A.length base});
+    offset: (offset: SZ.t {SZ.v offset <= A.length base});
+}
+
+[@@erasable]
+noeq
+type array elt = {
+  array_base: t elt;
+  array_len: (array_len: SZ.t {SZ.v array_base.offset + SZ.v array_len <= SZ.v array_base.glen});
+  array_perm: perm;
+}
+
+let array_len x : GTot SZ.t = x.array_len
+
+let array_length x : GTot nat = SZ.v (array_len x)
+
+let array_perm x = x.array_perm
+
+[@@erasable]
+noeq
+type v t = {
+  v_array: array t;
+  v_contents: Seq.lseq t (array_length v_array);
+}
+
+let array_of x = x.v_array
+let contents_of
+    #elt (x: v elt)
+: GTot (Seq.lseq elt (SZ.v (array_len (array_of x))))
+= x.v_contents
+
+let array_contents_inj
+    (#elt: Type0)
+    (v1 v2: v elt)
+: Lemma
+    (requires (array_of v1 == array_of v2 /\
+        contents_of v1 == contents_of v2
+    ))
+    (ensures v1 == v2)
+= ()
+
+let arrayptr1
+    (#elt: Type0)
+    (w: v elt)
+: vprop
+= A.pts_to_range w.v_array.array_base.base (SZ.v w.v_array.array_base.offset) (SZ.v w.v_array.array_base.offset + SZ.v w.v_array.array_len) #w.v_array.array_perm w.v_contents
+
+let arrayptr
+    (#elt: Type0)
+    (x: t elt)
+    (w: v elt)
+: vprop
+= arrayptr1 w **
+    pure (w.v_array.array_base == x)
+
+unfold
+let adjacent x1 x2 : prop =
+    x1.array_base.base == x2.array_base.base /\
+    x1.array_perm == x2.array_perm /\
+    SZ.v x1.array_base.offset + SZ.v x1.array_len == SZ.v x2.array_base.offset
+
+let merge #elt x1 x2 : Ghost (array elt)
+    (requires adjacent x1 x2)
+    (ensures (fun y ->
+        array_length y == array_length x1 + array_length x2 /\
+        array_perm y == array_perm x1 /\
+        array_perm y == array_perm x2
+    ))
+= {
+    array_base = x1.array_base;
+    array_len = x1.array_len `SZ.add` x2.array_len;
+    array_perm = x1.array_perm;
+}
+
+let merge_assoc x1 x2 x3 : Lemma
+        (requires (
+            (adjacent x1 x2 /\ adjacent x2 x3) \/
+            (adjacent x1 x2 /\ adjacent (merge x1 x2) x3) \/
+            (adjacent x2 x3 /\ adjacent x1 (merge x2 x3))
+        ))
+        (ensures (
+            adjacent x1 x2 /\ adjacent (merge x1 x2) x3 /\
+            adjacent x2 x3 /\ adjacent x1 (merge x2 x3) /\
+            merge (merge x1 x2) x3 == merge x1 (merge x2 x3)
+        ))
+= ()
+
+inline_for_extraction
+let instance0 : LA.array_ptr_step0 t array v = {
+    len = array_len;
+    array_perm = array_perm;
+    array_of = array_of;
+    contents_of = contents_of;
+    array_contents_inj = array_contents_inj;
+    arrayptr = arrayptr;
+    adjacent = adjacent;
+    merge = merge;
+    merge_assoc = merge_assoc;
+}
+
+```pulse
+ghost
+fn manurewrite
+    (p: vprop)
+    (q: vprop)
+requires (p **
+    pure (p == q)
+)
+ensures q
+{
+    rewrite p as q
+}
+```
+
+```pulse
+fn join
+    (_: unit)
+: LA.join_t #t #array #v instance0
+=
+    (#elt: Type0)
+    (al: t elt)
+    (ar: t elt)
+    (#vl: v elt)
+    (#vr: v elt)
+{
+    let res : Ghost.erased (v elt) = Ghost.hide (Mkv // FIXME: WHY WHY WHY can I not use record literals here?
+        (merge (array_of vl) (array_of vr))
+        (contents_of vl `Seq.append` contents_of vr)
+    );
+    rewrite (LA.arrayptr instance0 al vl) as (arrayptr al vl);
+    unfold (arrayptr al vl);
+    rewrite (arrayptr1 vl)
+        as (A.pts_to_range res.v_array.array_base.base (SZ.v res.v_array.array_base.offset) (SZ.v vr.v_array.array_base.offset) #res.v_array.array_perm vl.v_contents);
+    rewrite (LA.arrayptr instance0 ar vr) as (arrayptr ar vr);
+    unfold (arrayptr ar vr);
+    rewrite (arrayptr1 vr)
+        as (A.pts_to_range res.v_array.array_base.base (SZ.v vr.v_array.array_base.offset) (SZ.v res.v_array.array_base.offset + SZ.v res.v_array.array_len) #res.v_array.array_perm vr.v_contents);
+    A.pts_to_range_join res.v_array.array_base.base (SZ.v res.v_array.array_base.offset) (SZ.v vr.v_array.array_base.offset) (SZ.v res.v_array.array_base.offset + SZ.v res.v_array.array_len);
+    rewrite (A.pts_to_range res.v_array.array_base.base (SZ.v res.v_array.array_base.offset) (SZ.v res.v_array.array_base.offset + SZ.v res.v_array.array_len) #res.v_array.array_perm (vl.v_contents `Seq.append` vr.v_contents))
+        as (arrayptr1 res);
+    fold (arrayptr al res);
+    rewrite (arrayptr al res) as (LA.arrayptr instance0 al res);
+    res
+}
+```
+
+```pulse
+fn gsplit
+    (_: unit)
+: LA.gsplit_t #t #array #v instance0
+=
+    (#elt:Type0)
+    (x: t elt)
+    (i:SZ.t)
+    (#value:v elt)
+{
+    rewrite (LA.arrayptr instance0 x value) as (arrayptr x value);
+    unfold (arrayptr x value);
+    unfold (arrayptr1 value);
+    A.pts_to_range_prop value.v_array.array_base.base;
+    let vl : v elt = Mkv
+        (Mkarray
+            value.v_array.array_base
+            i
+            value.v_array.array_perm
+        )
+        (Seq.slice value.v_contents 0 (SZ.v i));
+    let vr : v elt = Mkv
+        (Mkarray
+            (Mkt
+                value.v_array.array_base.base
+                value.v_array.array_base.glen
+                (value.v_array.array_base.offset `SZ.add` i)
+            )
+            (value.v_array.array_len `SZ.sub` i)
+            value.v_array.array_perm
+        )
+        (Seq.slice value.v_contents (SZ.v i) (Seq.length value.v_contents));
+    let res : Ghost.erased (t elt) = Ghost.hide vr.v_array.array_base;
+    A.pts_to_range_split value.v_array.array_base.base (SZ.v value.v_array.array_base.offset) (SZ.v vr.v_array.array_base.offset) (SZ.v value.v_array.array_base.offset + SZ.v value.v_array.array_len);
+    rewrite
+        (A.pts_to_range value.v_array.array_base.base (SZ.v value.v_array.array_base.offset) (SZ.v vr.v_array.array_base.offset) #value.v_array.array_perm (Seq.slice value.v_contents 0 (SZ.v vr.v_array.array_base.offset - SZ.v value.v_array.array_base.offset)))
+        as (arrayptr1 vl);
+    fold (arrayptr x vl);
+    rewrite (arrayptr x vl) as (LA.arrayptr instance0 x vl);
+    rewrite
+        (A.pts_to_range value.v_array.array_base.base (SZ.v vr.v_array.array_base.offset) (SZ.v value.v_array.array_base.offset + SZ.v value.v_array.array_len) #value.v_array.array_perm (Seq.slice value.v_contents (SZ.v vr.v_array.array_base.offset - SZ.v value.v_array.array_base.offset) (Seq.length value.v_contents)))
+        as (arrayptr1 vr);
+    fold (arrayptr res vr);
+    rewrite (arrayptr res vr) as (LA.arrayptr instance0 res vr);
+    res
+}
+```
+
+inline_for_extraction
+```pulse
+fn split'
+    (_: unit)
+: LA.split_t #t #array #v instance0
+=
+    (#elt:Type)
+    (x: t elt)
+    (i: SZ.t)
+    (x': Ghost.erased (t elt))
+    (#vl: Ghost.erased (v elt))
+    (#vr: Ghost.erased (v elt))
+{
+    rewrite (LA.arrayptr instance0 x vl) as (arrayptr x vl);
+    unfold (arrayptr x vl);
+    fold (arrayptr x vl);
+    rewrite (arrayptr x vl) as (LA.arrayptr instance0 x vl);
+    rewrite (LA.arrayptr instance0 x' vr) as (arrayptr x' vr); 
+    unfold (arrayptr x' vr);
+    let res = Mkt
+        x.base
+        x.glen
+        (x.offset `SZ.add` i);
+    fold (arrayptr res vr);
+    rewrite (arrayptr res vr) as (LA.arrayptr instance0 res vr);
+    res
+}
+```
+
+inline_for_extraction
+```pulse
+fn index
+    (_: unit)
+: LA.index_t #t #array #v instance0
+=
+    (#elt:Type)
+    (r: t elt)
+    (i: SZ.t)
+    (#value: Ghost.erased (v elt))
+{
+    rewrite (LA.arrayptr instance0 r value) as (arrayptr r value);
+    unfold (arrayptr r value);
+    rewrite (arrayptr1 value)
+        as (A.pts_to_range r.base (SZ.v value.v_array.array_base.offset) (SZ.v value.v_array.array_base.offset + SZ.v value.v_array.array_len) #value.v_array.array_perm value.v_contents);
+    let y = A.pts_to_range_index r.base (r.offset `SZ.add` i);
+    rewrite (A.pts_to_range r.base (SZ.v value.v_array.array_base.offset) (SZ.v value.v_array.array_base.offset + SZ.v value.v_array.array_len) #value.v_array.array_perm value.v_contents)
+        as (arrayptr1 value);
+    fold (arrayptr r value);
+    rewrite (arrayptr r value) as  (LA.arrayptr instance0 r value);
+    y
+}
+```
+
+inline_for_extraction
+```pulse
+fn upd
+    (_: unit)
+: LA.upd_t #t #array #v instance0
+=
+    (#elt:Type)
+    (r: t elt)
+    (i:SZ.t)
+    (x:elt)
+    (#value: Ghost.erased (v elt))
+{
+    rewrite (LA.arrayptr instance0 r value) as (arrayptr r value);
+    unfold (arrayptr r value);
+    rewrite (arrayptr1 value)
+        as (A.pts_to_range r.base (SZ.v value.v_array.array_base.offset) (SZ.v value.v_array.array_base.offset + SZ.v value.v_array.array_len) #full_perm value.v_contents);
+    A.pts_to_range_upd r.base (r.offset `SZ.add` i) x;
+    with contents' . assert (A.pts_to_range r.base (SZ.v value.v_array.array_base.offset) (SZ.v value.v_array.array_base.offset + SZ.v value.v_array.array_len) #full_perm contents');
+    let value' : Ghost.erased (v elt) = Ghost.hide (Mkv
+        value.v_array
+        contents'        
+    );
+    rewrite (A.pts_to_range r.base (SZ.v value.v_array.array_base.offset) (SZ.v value.v_array.array_base.offset + SZ.v value.v_array.array_len) #full_perm contents')
+        as (arrayptr1 value');
+    fold (arrayptr r value');
+    rewrite (arrayptr r value') as (LA.arrayptr instance0 r value');
+    value'
+}
+```
+
+let set_array_perm
+    (#elt: Type)
+    (a: array elt)
+    (p: perm)
+:   Ghost (array elt)
+        (requires True)
+        (ensures (fun y -> instance0.len y == instance0.len a /\
+            instance0.array_perm y == p))
+= {a with
+    array_perm = p;
+}
+
+let set_array_perm_idem
+    (#elt: Type)
+    (a: array elt)
+    (p1: perm)
+    (p2: perm)
+:   Lemma
+    (set_array_perm (set_array_perm a p1) p2 == set_array_perm a p2)
+= ()
+
+let set_array_perm_eq
+    (#elt: Type)
+    (a: array elt)
+:   Lemma
+    (set_array_perm a (instance0.array_perm a) == a)
+= ()
+
+let set_array_perm_adjacent
+    (#elt: Type)
+    (a1: array elt)
+    (a2: array elt)
+    (p: perm)
+:   Lemma
+    (requires (instance0.adjacent a1 a2))
+    (ensures (
+        LA.merge_into instance0 (set_array_perm a1 p) (set_array_perm a2 p) (set_array_perm (instance0.merge a1 a2) p)
+    ))
+= ()
+
+let seq_slice_full (#elt: Type) (x: Seq.seq elt) : Lemma
+    (x == Seq.slice x 0 (Seq.length x))
+= assert (x `Seq.equal` Seq.slice x 0 (Seq.length x))
+
+inline_for_extraction
+```pulse
+fn copy
+    (_: unit)
+: LA.copy_t #t #array #v instance0
+=
+    (#elt: Type0)
+    (ain: t elt)
+    (aout: t elt)
+    (len: SZ.t)
+    (#vin: Ghost.erased (v elt))
+    (#vout: Ghost.erased (v elt))
+{
+    // FIXME: expose pts_to_range_memcpy in Pulse.Lib.Array
+    seq_slice_full vin.v_contents;
+    let mut pi = 0sz;
+    while
+        (
+            let i = !pi;
+            (i `SZ.lt` len)
+        )
+    invariant cont . exists i vout' .
+        pts_to pi i **
+        LA.arrayptr instance0 ain vin ** LA.arrayptr instance0 aout vout' ** pure (
+            instance0.array_of vout' == instance0.array_of vout /\
+            LA.length instance0 (instance0.array_of vin) == LA.length instance0 (instance0.array_of vout) /\
+            SZ.v i <= SZ.v len /\
+            Seq.slice (instance0.contents_of vout') 0 (SZ.v i) `Seq.equal` Seq.slice (instance0.contents_of vin) 0 (SZ.v i) /\
+            cont == (SZ.v i < SZ.v len)
+        )
+    {
+        let i = !pi;
+        let x = index () ain i;
+        let prf = upd () aout i x;
+        pi := (i `SZ.add` 1sz);
+        Seq.lemma_split (Seq.slice prf.v_contents 0 (SZ.v i + 1)) (SZ.v i);
+        Seq.lemma_split (Seq.slice vin.v_contents 0 (SZ.v i + 1)) (SZ.v i);
+        ()
+    };
+    with vout' . assert (LA.arrayptr instance0 aout vout');
+    seq_slice_full vout'.v_contents;
+    Ghost.hide vout'
+}
+```
+
+inline_for_extraction
+let instance1: LA.array_ptr_step1 instance0 = {
+    join = join ();
+    gsplit = gsplit ();
+    split' = split' ();
+    index = index ();
+    upd = upd ();
+    set_array_perm = set_array_perm;
+    set_array_perm_idem = set_array_perm_idem;
+    set_array_perm_eq = set_array_perm_eq;
+    set_array_perm_adjacent = set_array_perm_adjacent;
+    copy = copy ();
+}
